isabelletarjan.thy
@@ -1,6 +1,6 @@
 theory isabelletarjan
   imports Main
-  "~~/src/HOL/Library/State_Monad"
+  "State_Monad_HL"
 
 begin
 
@@ -28,71 +28,31 @@ record 'v env =
   sn    :: nat
   num   :: "'v \<Rightarrow> int"
 
-text\<open>Helper methods for manipulating the environment fields hided in the Monad\<close>
-definition return:: "'a \<Rightarrow> ('b, 'a) state" where "return = State_Monad.return"
-definition get:: "('a env, 'a env) state" where "get = State (\<lambda>x. (x,x))"
-definition put:: "'a env \<Rightarrow> ('a env, unit) state" where "put x = State (\<lambda>_. ((),x))"
+subsection\<open>update functions\<close>
+definition black_Env:: "'v env \<Rightarrow> 'v set \<Rightarrow> 'v env" where "black_Env s v = s \<lparr> black := v \<rparr>"
+definition gray_Env:: "'v env \<Rightarrow> 'v set \<Rightarrow> 'v env" where "gray_Env s v = s \<lparr> gray := v \<rparr>"
+definition stack_Env:: "'v env \<Rightarrow> 'v list \<Rightarrow> 'v env" where "stack_Env s v = s \<lparr> stack := v \<rparr>"
+definition sccs_Env:: "'v env \<Rightarrow> 'v set set \<Rightarrow> 'v env" where "sccs_Env s v = s \<lparr> sccs := v \<rparr>"
+definition sn_Env:: "'v env \<Rightarrow> nat \<Rightarrow> 'v env" where "sn_Env s v = s \<lparr> sn := v \<rparr>"
+definition num_Env:: "'v env \<Rightarrow> ('v \<Rightarrow> int) \<Rightarrow> 'v env" where "num_Env s v = s \<lparr> num := v \<rparr>"
 
-definition get_gen:: "('a env \<Rightarrow> 'b) \<Rightarrow> ('a env, 'b) state" where "get_gen acc = do { x \<leftarrow> get; return (acc  x)}"
+theorem put_black_rule: "spec (\<lambda>x. p () (x \<lparr> black := v \<rparr>)) (put black_Env v) p"
+  by (simp add: spec_def put_def get_state_def put_state_def black_Env_def)
 
-definition get_black:: "('a env, 'a set) state" where "get_black = do { x \<leftarrow> get; return (black  x) }" 
-definition get_gray:: "('a env, 'a set) state" where "get_gray = do { x \<leftarrow> get; return (gray x) }" 
-definition get_stack:: "('a env, 'a list) state" where "get_stack = do { x \<leftarrow> get; return (stack x) }" 
-definition get_sccs:: "('a env, 'a set set) state" where "get_sccs = do { x \<leftarrow> get; return (sccs x) }" 
-definition get_sn:: "('a env, nat) state" where "get_sn = do { x \<leftarrow> get; return (sn x) }" 
-definition get_num:: "('a env, 'a \<Rightarrow> int) state" where "get_num = do { x \<leftarrow> get; return (num x) }" 
+theorem put_gray_rule: "spec (\<lambda>x. p () (x \<lparr> gray := v \<rparr>)) (put gray_Env v) p"
+  by (simp add: spec_def put_def get_state_def put_state_def gray_Env_def)
 
-definition set_black:: "'a env \<Rightarrow> 'a set \<Rightarrow> 'a env" where "set_black v x =  
-\<lparr>            black = x,
-             gray = gray v,
-             stack = stack v,
-             sccs = sccs v,
-             sn = sn v,
-             num = num v \<rparr>"
-definition set_gray:: "'a env \<Rightarrow> 'a set \<Rightarrow> 'a env" where "set_gray v x =
-\<lparr>            black = black v,
-             gray = x,
-             stack = stack v,
-             sccs = sccs v,
-             sn = sn v,
-             num = num v \<rparr>"
-definition set_stack:: "'a env \<Rightarrow> 'a list \<Rightarrow> 'a env" where "set_stack v x = 
-\<lparr>            black = black v,
-             gray = gray v,
-             stack = x,
-             sccs = sccs v,
-             sn = sn v,
-             num = num v \<rparr>"
-definition set_sccs:: "'a env \<Rightarrow> 'a set set \<Rightarrow> 'a env" where "set_sccs v x = 
-\<lparr>            black = black v,
-             gray = gray v,
-             stack = stack v,
-             sccs = x,
-             sn = sn v,
-             num = num v \<rparr>"
-definition set_sn:: "'a env \<Rightarrow> nat \<Rightarrow> 'a env" where "set_sn v x = 
-\<lparr>            black = black v,
-             gray = gray v,
-             stack = stack v,
-             sccs = sccs v,
-             sn = x,
-             num = num v \<rparr>"
-definition set_num:: "'a env \<Rightarrow> ('a \<Rightarrow> int) \<Rightarrow> 'a env" where "set_num v x = 
-\<lparr>            black = black v,
-             gray = gray v,
-             stack = stack v,
-             sccs = sccs v,
-             sn = sn v,
-             num = x \<rparr>"
+theorem put_stack_rule: "spec (\<lambda>x. p () (x \<lparr> stack := v \<rparr>)) (put stack_Env v) p"
+  by (simp add: spec_def put_def get_state_def put_state_def stack_Env_def)
 
-definition put_black:: "'a set \<Rightarrow> ('a env, unit) state" where "put_black x = do { v \<leftarrow> get; put (set_black v x) }"
-definition put_gray:: "'a set \<Rightarrow> ('a env, unit) state" where "put_gray x = do { v \<leftarrow> get; put (set_gray v x) }"
-definition put_stack:: "'a list \<Rightarrow> ('a env, unit) state" where "put_stack x = do { v \<leftarrow> get; put (set_stack v x) }"
-definition put_sccs:: "'a set set \<Rightarrow> ('a env, unit) state" where "put_sccs x = do { v \<leftarrow> get; put (set_sccs v x) }"
-definition put_sn:: "nat \<Rightarrow> ('a env, unit) state" where "put_sn x = do { v \<leftarrow> get; put (set_sn v x) }"
-definition put_num:: "('a \<Rightarrow> int) \<Rightarrow> ('a env, unit) state" where "put_num x = do { v \<leftarrow> get; put (set_num v x) }"
+theorem put_sccs_rule: "spec (\<lambda>x. p () (x \<lparr> sccs := v \<rparr>)) (put sccs_Env v) p"
+  by (simp add: spec_def put_def get_state_def put_state_def sccs_Env_def)
 
-definition skip:: "('a env, unit) state" where "skip = State (\<lambda>x. ((),x))"
+theorem put_sn_rule: "spec (\<lambda>x. p () (x \<lparr> sn := v \<rparr>)) (put sn_Env v) p"
+  by (simp add: spec_def put_def get_state_def put_state_def sn_Env_def)
+
+theorem put_num_rule: "spec (\<lambda>x. p () (x \<lparr> num := v \<rparr>)) (put num_Env v) p"
+  by (simp add: spec_def put_def get_state_def put_state_def num_Env_def)
 
 definition colored where
   "colored e \<equiv> black e \<union> gray e"
@@ -230,46 +190,104 @@ text \<open>
   It is also added to the set of gray nodes.
 \<close>
 
+
 definition insert_black:: "'v \<Rightarrow> ('v env, unit) state" where
 "insert_black x \<equiv> do{
-       b \<leftarrow> get_gen black;
-       b \<leftarrow> return (insert x b);
-       put_black b
+       b \<leftarrow> get black;
+       put black_Env (insert x b)
     }"
 
-definition insert_sccs:: "'v list \<Rightarrow> ('v env, unit) state" where
+subsubsection\<open>Insert black spec - lemmas:\<close>
+definition insert_black_pre:: "'v env \<Rightarrow> 'v \<Rightarrow> 'v env \<Rightarrow> bool " where
+"insert_black_pre e x s \<equiv> s = e
+                          \<and> x \<notin> (black e)"
+
+definition insert_black_post:: "'v env \<Rightarrow> 'v \<Rightarrow>  'v env \<Rightarrow> bool " where
+"insert_black_post e x e2 \<equiv> x \<notin> (black e)
+                            \<and> x \<in> black e2
+                            \<and> sccs e = sccs e2
+                            \<and> sn e = sn e2
+                            \<and> gray e = gray e2
+                            \<and> num e = num e2
+                            \<and> card (black e) \<le> card (black e2)"
+
+lemma black_inc: "spec (insert_black_pre e x) (insert_black x) (GG (insert_black_post e x))"
+  unfolding insert_black_pre_def GG_def insert_black_post_def
+  apply(simp add: insert_black_def)
+  apply(intro get_rule; intro allI; simp)
+  apply(simp add: spec_def put_def get_state_def put_state_def black_Env_def)
+  by (metis card_infinite card_insert_le card_mono eq_iff subset_insertI)
+
+
+definition insert_sccs where
 "insert_sccs x \<equiv> do{
-       scc \<leftarrow> get_gen sccs;
-       scc \<leftarrow> return (insert (set x) scc);
-       put_sccs scc
+       scc \<leftarrow> get sccs;
+       put sccs_Env (insert (set x) scc)
     }"
+
+subsubsection\<open>Insert sccs spec - lemmas:\<close>
+
 
 definition insert_gray:: "'v \<Rightarrow> ('v env, unit) state" where
 "insert_gray x \<equiv> do{
-       g \<leftarrow> get_gen gray;
-       g \<leftarrow> return (insert x g);
-       put_gray g
+       g \<leftarrow> get gray;
+       put gray_Env (insert x g)
     }"
+
+subsubsection\<open>Insert black spec - lemmas:\<close>
+definition insert_gray_pre:: "'v env \<Rightarrow> 'v \<Rightarrow> 'v env \<Rightarrow> bool " where
+"insert_gray_pre e x s \<equiv> s = e
+                          \<and> x \<notin> (gray e)
+                          \<and> x \<in> vertices"
+
+definition insert_gray_post:: "'v env \<Rightarrow> 'v \<Rightarrow>  'v env \<Rightarrow> bool " where
+"insert_gray_post e x e2 \<equiv>  x \<in> vertices
+                            \<and> x \<notin> (gray e)
+                            \<and> x \<in> gray e2
+                            \<and> sccs e = sccs e2
+                            \<and> sn e = sn e2
+                            \<and> black e = black e2
+                            \<and> num e = num e2
+                            \<and> card (gray e) \<le> card (gray e2)"
+
+lemma gray_inc: "spec (insert_gray_pre e x) (insert_gray x) (GG (insert_gray_post e x))"
+  unfolding insert_gray_pre_def GG_def insert_gray_post_def
+  apply(simp add: insert_gray_def)
+  apply(intro get_rule; intro allI; simp)
+  apply(simp add: spec_def put_def get_state_def put_state_def gray_Env_def)
+  by (metis card_infinite card_insert_le card_mono eq_iff subset_insertI)
+
 
 definition insert_stack:: "'v  \<Rightarrow> ('v env, unit) state" where
 "insert_stack x \<equiv> do {
-       st \<leftarrow> get_gen stack;
-       st \<leftarrow> return (x # st);
-       put_stack st
+       st \<leftarrow> get stack;
+       put stack_Env (x # st)
     }"
 
 definition count_up_sn:: "('v env, unit) state" where
 "count_up_sn \<equiv> do {
-      sn \<leftarrow> get_gen sn;
-      put_sn (sn + 1)
+      sn \<leftarrow> get sn;
+      put sn_Env (sn + 1)
 }"
+
+subsubsection\<open>count_up_sn lemma\<close>
+definition count_up_pre:: "'v env \<Rightarrow> 'v env \<Rightarrow> bool" where
+"count_up_pre e s \<equiv> e = s \<and>
+                    sn e \<le> (card vertices)"
+
+definition count_up_post:: "'v env \<Rightarrow> 'v env \<Rightarrow> bool" where
+"count_up_post e e2 \<equiv> sn e < sn e2"
+
+lemma count_up_spec: "spec (count_up_pre e) count_up_sn (GG (count_up_post e))"
+  unfolding count_up_pre_def GG_def count_up_post_def
+  apply(simp add: count_up_sn_def)
+  apply(intro get_rule; intro allI; simp)
+  by(simp add: spec_def put_def get_state_def sn_Env_def put_state_def)
 
 definition update_num:: "'v \<Rightarrow> ('v env, unit) state" where
 "update_num x \<equiv> do {
-      num \<leftarrow> get_gen num;
-      sn \<leftarrow> get_gen sn;
-      num \<leftarrow> return (num (x := int(sn)));
-      put_num num
+      (num, sn) \<leftarrow> get (\<lambda>e. (num e, sn e));
+      put num_Env (num (x := int(sn)))
 }"
 
 definition add_stack_incr:: "'v \<Rightarrow> ('v env, unit) state" where
@@ -280,6 +298,32 @@ definition add_stack_incr:: "'v \<Rightarrow> ('v env, unit) state" where
     update_num x
   }"
 
+subsubsection\<open>Add_stack_incr lemmas\<close>
+definition add_stack_incr_pre:: "'v \<Rightarrow> 'v env \<Rightarrow> 'v env \<Rightarrow> bool" where
+"add_stack_incr_pre x e s \<equiv> e = s
+                          \<and> x \<in> vertices
+                          \<and> x \<notin> gray e
+                          \<and> x \<notin> black e
+                          \<and> x \<notin> set(stack e)
+                          \<and> (num e) x = -1"
+
+definition add_stack_incr_post:: "'v \<Rightarrow> 'v env \<Rightarrow> 'v env \<Rightarrow> bool" where
+"add_stack_incr_post x e e2 \<equiv> 
+                          x \<in> gray e2
+                          \<and> x \<in> vertices
+                          \<and> x \<in> black e2
+                          \<and> x \<in> set(stack e2)
+                          \<and> (num e2) x \<noteq> -1"
+
+lemma add_stack_incr_spec: "spec (add_stack_incr_pre x e) (add_stack_incr x) (GG (add_stack_incr_post x e))"
+  unfolding add_stack_incr_pre_def GG_def add_stack_incr_post_def
+  apply(simp add:add_stack_incr_def)
+  apply(simp add: insert_gray_def)
+  apply(intro get_rule; intro allI; simp)
+  apply(simp add: gray_Env_def put_def get_def get_state_def put_state_def)
+  apply (intro seq_rule[of _ _ "(\<lambda>_ e2. x \<in> gray e2 \<and> x \<in> vertices \<and> x \<in> black e2 \<and> x \<in> set (stack e2) \<and> num e2 x \<noteq> - 1)"])
+sorry
+
 text \<open>
   Add vertex @{text x} to the set of black vertices in @{text e}
   and remove it from the set of gray vertices.
@@ -288,27 +332,27 @@ text \<open>
 definition add_black:: "'v \<Rightarrow> ('v env, unit) state" where
   "add_black x =   do{
                            insert_black x;
-                           gr \<leftarrow> get_gen gray;
+                           gr \<leftarrow> get gray;
                            gr \<leftarrow> return (gr - {x});
-                           put_gray gr
+                           put gray_Env gr
                         }"
 
 definition update_list where
 "update_list l \<equiv>    
   do{   
-      n \<leftarrow> get_gen num;
+      n \<leftarrow> get num;
       let n1 = set_infty l n;
-      put_num n1  
+      put num_Env n1  
   }"
 
 definition update_env  where
   "update_env x =   
   do{
       insert_black x;
-      st \<leftarrow> get_gen stack;
+      st \<leftarrow> get stack;
       let (l,r) = split_list x st;
       insert_sccs l;
-      put_stack r;
+      put stack_Env r;
       update_list l
     }"
 
@@ -333,7 +377,7 @@ function (domintros) dfs1 and dfs where
   "dfs1 x = do {
     add_stack_incr x;
     let n1 = dfs (successors x);
-    snum \<leftarrow> get_gen sn;
+    snum \<leftarrow> get sn;
     if int n1 < int snum then do{
       add_black x;
       n1
@@ -347,7 +391,7 @@ function (domintros) dfs1 and dfs where
     a \<leftarrow> (if roots = {} then (return \<infinity>)
     else do {
        let x = (SOME x. x \<in> roots);
-       num \<leftarrow> get_num;
+       num \<leftarrow> get num;
        let res1 = (if num x > 0 then (num x) else (dfs1 x));
        let res2 = dfs (roots - {x});
        (min res1 res2)
